#### 德摩根式

$\overline{xy}$  =  $\bar{x} + \bar{y}$

$\overline{(x+y)}$  =  $\bar{x}$ · $\bar{y}$

#### 分配律

$(x+y)·z = xz + yz$ 

$x+yz = (x+y)·(x+z)$

###### 		推导：$(x+y)·(x+z) = (x+xy+xz)+yz = x(1+y+z)+yz = x + yz$

#### 吸收律

|                    A(A+B) = A                    |              A+A·B = A               |
| :----------------------------------------------: | :----------------------------------: |
|             **A·($\bar{A}$+B) = AB**             |      **A + $\bar{A}$·B = A+B**       |
| **(A+B)($\bar{A}$+C)(B+C) = (A+B)($\bar{A}$+C)** | **AB+$\bar{A}$C+BC = AB+$\bar{A}$C** |

[推导](https://zhuanlan.zhihu.com/p/392457877) 

$A·(\bar{A}+B) = A·\bar{A} + A·B = 0 + A·B = AB$

$A + \bar{A}·B = (A+\bar{A})·(A+B)(分配律2) = 1·(A+B) = A+B$

$(A+B)(\bar{A}+C)(B+C)$

##### 		= $(A+B)(\bar{A}+C)(0+B+C)$ 

​		= $(A+B)(\bar{A}+C)(A·\bar{A}+B+C)$ 

##### 		= $(A+B)(\bar{A}+C)(A+(B+C))(\bar{A}+(B+C))$	(分配律2)

​		= $(A+B)(\bar{A}+C)((A+B)+C)((\bar{A}+C)+B)$

​		= $(A+B)(\bar{A}+C)$

$AB+\bar{A}C+BC$

​		= $AB + \bar{A}C + 1·BC$

​		= $AB + \bar{A}C + (A+\bar{A})·BC$

​		= $AB + \bar{A}C + ABC + \bar{A}BC$

​		= $AB + \bar{A}C$
